template-coq/theories/kernel/uGraph.v
@@ -174,11 +174,11 @@ Section UGraph.
   Definition exists_strictly_bigger (e1 : Universe.Expr.t) (u2 : Universe.t) : bool :=
     Universe.existsb (check_lt_level_expr e1) u2.
 
-  Definition check_leq (u1 u2 : Universe.t) : bool :=
-    Universe.for_all (fun e => exists_bigger_or_eq e u2) u1.
+  Definition check_leq `{cf : checker_flags} (u1 u2 : Universe.t) : bool :=
+    (negb check_univs) || Universe.for_all (fun e => exists_bigger_or_eq e u2) u1.
 
-  Definition check_lt `{cf : checker_flags} (u1 u2 : Universe.t) : bool :=
-    (negb check_univs) || Universe.for_all (fun e => exists_strictly_bigger e u2) u1.
+  Definition check_lt (u1 u2 : Universe.t) : bool :=
+    Universe.for_all (fun e => exists_strictly_bigger e u2) u1.
 
   (* true is all is ok *)
   Definition no_universe_inconsistency : bool :=
